infrastructure for mixed-mode proofs

floyd/mixed_mode.v
@@ -1,11 +1,77 @@
 Set Warnings "-notation-overridden,-custom-entry-overridden,-hiding-delimiting-key".
-From VST.typing Require Import programs own array function adequacy.
+From VST.typing Require Import programs singleton own array function adequacy.
 Set Warnings "notation-overridden,custom-entry-overridden,hiding-delimiting-key".
 Require Import VST.floyd.proofauto.
+
+Definition to_address (v : val) := option.default (1%positive, Ptrofs.zero) (type.val2adr v).
+
+Lemma to_address_eq v : isptr v → adr2val (to_address v) = v.
+Proof. by destruct v. Qed.
+
+Arguments nested_field_offset {_} _ _ /.
+Arguments cenv_cs : simpl never.
 
 Section mixed.
 
 Context `{!VSTGS OK_ty Σ} {cs : compspecs}.
+
+Lemma unfold_own_type cty v l t : ty_has_op_type t cty MCNone → v ◁ᵥ|tptr cty| l @ &own t ⊣⊢ ⌜l = to_address v⌝ ∧ ∃ a, data_at Tsh cty a v ∗ a ◁ᵥ|cty| t.
+Proof.
+  intros.
+  rewrite /frac_ptr; simpl_type.
+  rewrite /repinject /= -bi.persistent_and_affinely_sep_l.
+  eapply pure_equiv; first apply bi.and_elim_l.
+  { iIntros "(-> & % & H & _)"; rewrite data_at_isptr.
+    iDestruct "H" as "(% & _)"; rewrite to_address_eq //. }
+  intros ->; rewrite !bi.pure_True //; last by destruct l.
+  rewrite !bi.True_and /data_at /field_at /at_offset /=.
+  setoid_rewrite Ptrofs.add_zero.
+  iSplit.
+  - iIntros "H".
+    iDestruct (ty_aligned with "H") as %?; first done.
+    iDestruct (ty_deref with "H") as (?) "($ & $)"; done.
+  - iIntros "(% & (% & H) & ?)".
+    iApply (ty_ref with "[//] H"); done.
+Qed.
+
+Lemma unfold_own_type0 cty v t : ty_has_op_type t cty MCNone → v ◁ᵥ|tptr cty| &own t ⊣⊢ ∃ a, data_at Tsh cty a v ∗ a ◁ᵥ|cty| t.
+Proof.
+  intros.
+  rewrite /ty_of_rty; simpl_type.
+  setoid_rewrite unfold_own_type; last done.
+  iSplit.
+  - iIntros "(% & -> & $)".
+  - iIntros "(% & H & $)".
+    rewrite {1}data_at_isptr; iDestruct "H" as (?) "$"; eauto.
+Qed.
+
+Lemma unfold_int_type a k : repable_signed k → a ◁ᵥ|tint| k @ int.int tint ⊣⊢ <affine> ⌜a = Vint (Int.repr k)⌝.
+Proof.
+  intros; rewrite /int.int; simpl_type.
+  iSplit.
+  - iIntros "(_ & _ & %Hk)".
+    destruct a; inv Hk.
+    rewrite Int.repr_signed //.
+  - iIntros (->); iPureIntro.
+    rewrite /= Int.signed_repr //.
+Qed.
+
+Lemma unfold_value_type cty a v : type_is_volatile cty = false → value_fits cty (valinject cty v) →
+  a ◁ᵥ|cty| value cty v ⊣⊢ <affine> ⌜a = valinject cty v⌝.
+Proof.
+  intros; rewrite /value; simpl_type.
+  iPureIntro; split; try tauto.
+  intros ->; done.
+Qed.
+
+Lemma unfold_value_ptr_type cty a v : is_pointer_or_null v →
+  a ◁ᵥ|tptr cty| value (tptr cty) v ⊣⊢ <affine> ⌜a = v⌝.
+Proof.
+  intros; apply (unfold_value_type (tptr cty)); try done.
+  rewrite value_fits_eq /=.
+  intros _; simpl.
+  rewrite andb_false_r //.
+Qed.
 
 (* for now, fix to const type *)
 Program Definition fn_params_pre' {A} fn params fp : @dtfr Σ (ConstType A) -n> (genviron * list val) -d> mpred := λne x,
